\documentclass[a4paper,14pt]{extarticle}
% Стандартные формульные пакеты
\usepackage{float,amsmath,esint,amsfonts,wrapfig,bbm}
\usepackage{indentfirst}
\usepackage[usenames]{color}
\usepackage{multirow}
%выставляем поля
\usepackage[left=2cm,right=2cm,top=2cm,bottom=2cm,bindingoffset=0cm]{geometry}
% Русский текст в формулах
\usepackage{mathtext}
% Подключение русского языка
\usepackage[T2A]{fontenc}
\usepackage[english,russian]{babel}
\usepackage[utf8]{inputenc}
% Рисунки
\usepackage{graphicx,caption,subcaption}
% Landscape page
\usepackage{lscape}
\renewcommand{\arraystretch}{1.1}

\newcommand{\mymean}[3]{\left\langle #1 \left| #2 \right| #3 \right\rangle}
\newcommand{\myint}[2]{\langle #1 | #2 \rangle}
\newcommand{\myexp}[1]{\text{exp}\left( #1 \right)}
\begin{document}
$$V = \frac{1}{2}m\omega^2x^2,\ \dot{q}_k=\frac{p_k}{m},\ \dot{p}_k=-\left.\frac{\partial V}{\partial x}\right|_{q_k}=-m\omega^2q_k $$
$$g_k = N\myexp{\frac{1}{\hbar}\left(-\frac{1}{2}m\omega(x-q_k)^2+ip_k(x-q_k)\right)} = \myexp{\frac{1}{\hbar}\left(-\frac{1}{2}m\omega x^2 + \xi_kx + \eta_k\right)}$$
$$\xi_k = m\omega q_k + ip_k,\ \eta_k = \ln{N} - \frac{1}{2}m\omega q_k^2 - iq_kp_k$$
$$\dot{\xi}_k=m\omega\dot{q}_k+i\dot{p}_k=\omega p_k - im\omega^2q_k = -i\omega(m\omega q_k + ip_k)=-i\omega\xi_k$$
$$\dot{\eta}_k=-m\omega q_k\dot{q}_k-i(\dot{q}_kp_k+q_k\dot{p}_k)=-\dot{q}_k(m\omega q_k + ip_k)-iq_k\dot{p}_k=-\frac{p_k\xi_k}{m}+im\omega^2 q_k^2$$
$$\tau_{mk}=\myint{g_m}{\dot{g}_k}=\frac{1}{\hbar}\mathbbm{S}_{mk}\left( \dot{\eta}_k+\dot{\xi}_k\frac{\xi_k+\xi_m^*}{2m\omega}\right)=%
				   \frac{1}{\hbar}\mathbbm{S}_{mk}\left(im\omega^2 q_k^2-\frac{p_k\xi_k}{m}-i\frac{\xi_k^2+\xi_k\xi_m^*}{2m}\right)=$$
$$=\frac{1}{\hbar}\mathbbm{S}_{mk}\left(im\omega^2 q_k^2 - \frac{i\xi_k\xi_m^*}{2m} - \frac{i\xi_k(\xi_k-2ip_k)}{2m}\right)=%
   \frac{1}{\hbar}\mathbbm{S}_{mk}\left(im\omega^2 q_k^2 - \frac{i\xi_k\xi_m^*}{2m} - \frac{i|\xi_k|^2}{2m} \right)=$$
$$=\frac{1}{\hbar}\mathbbm{S}_{mk}\left(im\omega^2 q_k^2 - \frac{i\xi_k\xi_m^*}{2m} - \frac{i(m^2\omega^2q_k^2 + p_k^2)}{2m} \right)=%
   \frac{1}{\hbar}\mathbbm{S}_{mk}\left(\frac{i}{2}m\omega^2q_k^2 - \frac{ip_k^2}{2m} - \frac{i\xi_k\xi_m^*}{2m}\right)$$
$$\mathbbm{H}_{mk} = \mymean{g_m}{\hat{T}}{g_k} + \frac{1}{2}m\omega^2\mymean{g_m}{x^2}{g_k} =%
		     -\frac{\hbar^2}{2m}\mymean{g_m}{\frac{\partial^2}{\partial x^2}}{g_k} + \frac{1}{2}m\omega^2\mymean{g_k}{x^2}{g_m}=$$
$$=-\frac{\hbar^2}{2m}\mymean{g_m}{\frac{1}{\hbar}\frac{\partial}{\partial x} (-m\omega x + \xi_k)}{g_k} + \frac{1}{2}m\omega^2\mymean{g_k}{x^2}{g_m}=$$
$$=\frac{\hbar\omega}{2}\myint{g_m}{g_k} - \frac{1}{2m}\mymean{g_m}{(-m\omega x + \xi_k)^2}{g_k} + \frac{1}{2}m\omega^2\mymean{g_k}{x^2}{g_m}=$$
$$=\left(\frac{\hbar\omega}{2}-\frac{\xi_k^2}{2m}\right)\myint{g_m}{g_k}+\omega\xi_k\mymean{g_m}{x}{g_k}-%
	 \frac{1}{2}m\omega^2\mymean{g_m}{x^2}{g_k} + \frac{1}{2}m\omega^2\mymean{g_k}{x^2}{g_m}=$$
$$=\left(\left(\frac{\hbar\omega}{2}-\frac{\xi_k^2}{2m}\right)+\omega\xi_k\frac{(\xi_m^*+\xi_k)}{2m\omega}\right)\myint{g_m}{g_k}=%
   \left(\frac{\hbar\omega}{2}+\frac{\xi_m^*\xi_k}{2m}\right)\myint{g_m}{g_k}$$
$$\mathbbm{H}_{mk} - i\hbar\boldsymbol{\tau}_{mk} = \left( \frac{\hbar\omega}{2} + \frac{\xi_m^*\xi_k}{2m} + %
							   \frac{1}{2}m\omega^2q_k^2- \frac{p_k^2}{2m} -\frac{\xi_m^*\xi_k}{2m} \right)\myint{g_m}{g_k}=$$
$$=\left( \frac{\hbar\omega}{2} + \frac{1}{2}m\omega^2q_k^2 - \frac{p_k^2}{2m} \right)\mathbbm{S}_{mk}$$
$$( -i\mathbbm{S}^{-1}\left(\mathbbm{H}-i\hbar\boldsymbol{\tau}\right) )_{nk} = %
    -i\sum_m \mathbbm{S}^{-1}_{nm}\left( \mathbbm{H}_{mk} - i\hbar\boldsymbol{\tau}_{mk} \right) = $$
$$=\left( \frac{\hbar\omega}{2} +\frac{1}{2}m\omega^2q_k^2 - \frac{p_k^2}{2m} \right)\sum_m\mathbbm{S}^{-1}_{nm}\mathbbm{S}_{mk} = %
   \left( \frac{\hbar\omega}{2} +\frac{1}{2}m\omega^2q_k^2 - \frac{p_k^2}{2m} \right)\delta_{nk}$$
\end{document}
