$$V = \frac{1}{2}m\omega^2x^2,\ \dot{q}_k=\frac{p_k}{m},\ \dot{p}_k=-\left.\frac{\partial V}{\partial x}\right|_{q_k}=-m\omega^2q_k $$
$$g_k = N\myexp{\frac{1}{\hbar}\left(-\frac{1}{2}m\omega(x-q_k)^2+ip_k(x-q_k)\right)} = \myexp{\frac{1}{\hbar}\left(-\frac{1}{2}m\omega x^2 + \xi_kx + \eta_k\right)}$$
$$\xi_k = m\omega q_k + ip_k,\ \eta_k = \hbar\ln{N} - \frac{1}{2}m\omega q_k^2 - iq_kp_k$$
$$\dot{\xi}_k=m\omega\dot{q}_k+i\dot{p}_k=\omega p_k - im\omega^2q_k = -i\omega(m\omega q_k + ip_k)=-i\omega\xi_k$$
$$\dot{\eta}_k=-m\omega q_k\dot{q}_k-i(\dot{q}_kp_k+q_k\dot{p}_k)=-\dot{q}_k(m\omega q_k + ip_k)-iq_k\dot{p}_k=-\frac{p_k\xi_k}{m}+im\omega^2 q_k^2$$
$$\mathbbm{S}_{mk}=\myint{g_m}{g_k}=\int\myexp{\frac{1}{\hbar}\left(-m\omega x^2+(\xi_m^*+\xi_k)x+\eta_m^*+\eta_k\right)}\,dx=$$
$$=\int\myexp{\frac{1}{\hbar}\left(-m\omega\left[x-\frac{\xi_m^*+\xi_k}{2m\omega}\right]^2+\frac{(\xi_m^*+\xi_k)^2}{4m\omega}+%
				   \eta_m^*+\eta_k\right)}\,dx=$$
$$=\myexp{\frac{1}{\hbar}\left(\frac{(\xi_m^*+\xi_k)^2}{4m\omega}+\eta_m^*+\eta_k\right)}\int\myexp{-\frac{m\omega}{\hbar}y^2}\,dy=$$
$$=\myexp{\frac{1}{\hbar}\left(\frac{(\xi_m^*+\xi_k)^2}{4m\omega}+\eta_m^*+\eta_k\right)}\sqrt{\frac{\hbar\pi}{m\omega}}$$
$$\mathbbm{S}_{kk}= N^2 \sqrt{ \frac{\hbar\pi}{m\omega} }=1\ \Rightarrow\ N = \left(\frac{m\omega}{\hbar\pi}\right)^{1/4}$$
$$\mymean{g_m}{x}{g_k} = \int x\cdot\myexp{\frac{1}{\hbar}\left(-m\omega x^2+(\xi_m^*+\xi_k)x+\eta_m^*+\eta_k\right)}\,dx=$$
$$=\hbar\int\frac{\partial}{\partial(\xi_m^*+\xi_k)}\myexp{\frac{1}{\hbar}\left(-m\omega x^2 + (\xi_m^*+\xi_k)x+\eta_m^*+\eta_k\right)}\,dx$$
$$=\hbar\frac{\partial\mathbbm{S}_{mk}}{\partial(\xi_m^*+\xi_k)}=\frac{(\xi_m^*+\xi_k)}{2m\omega}\mathbbm{S}_{mk}$$
$$\mymean{g_m}{x^2}{g_k}=\int x^2\cdot\myexp{\frac{1}{\hbar}\left(-m\omega x^2+(\xi_m^*+\xi_k)x+\eta_m^*+\eta_k\right)}\,dx=$$
$$=\hbar^2\frac{\partial^2\mathbbm{S}_{mk}}{\partial(\xi_m^*+\xi_k)^2}=\frac{\hbar}{2m\omega}+\left(\frac{\xi_m^*+\xi_k}{2m\omega}\right)^2$$
$$\tau_{mk}=\myint{g_m}{\dot{g}_k}=\frac{1}{\hbar}\mathbbm{S}_{mk}\left( \dot{\eta}_k+\dot{\xi}_k\frac{\xi_k+\xi_m^*}{2m\omega}\right)=%
				   \frac{1}{\hbar}\mathbbm{S}_{mk}\left(im\omega^2 q_k^2-\frac{p_k\xi_k}{m}-i\frac{\xi_k^2+\xi_k\xi_m^*}{2m}\right)=$$
$$=\frac{1}{\hbar}\mathbbm{S}_{mk}\left(im\omega^2 q_k^2 - \frac{i\xi_k\xi_m^*}{2m} - \frac{i\xi_k(\xi_k-2ip_k)}{2m}\right)=%
   \frac{1}{\hbar}\mathbbm{S}_{mk}\left(im\omega^2 q_k^2 - \frac{i\xi_k\xi_m^*}{2m} - \frac{i|\xi_k|^2}{2m} \right)=$$
$$=\frac{1}{\hbar}\mathbbm{S}_{mk}\left(im\omega^2 q_k^2 - \frac{i\xi_k\xi_m^*}{2m} - \frac{i(m^2\omega^2q_k^2 + p_k^2)}{2m} \right)=%
   \frac{1}{\hbar}\mathbbm{S}_{mk}\left(\frac{i}{2}m\omega^2q_k^2 - \frac{ip_k^2}{2m} - \frac{i\xi_k\xi_m^*}{2m}\right)$$
$$\mathbbm{H}_{mk} = \mymean{g_m}{\hat{T}}{g_k} + \frac{1}{2}m\omega^2\mymean{g_m}{x^2}{g_k} =%
		     -\frac{\hbar^2}{2m}\mymean{g_m}{\frac{\partial^2}{\partial x^2}}{g_k} + \frac{1}{2}m\omega^2\mymean{g_m}{x^2}{g_k}=$$
$$=-\frac{\hbar^2}{2m}\mymean{g_m}{\frac{1}{\hbar}\frac{\partial}{\partial x} (-m\omega x + \xi_k)}{g_k} + \frac{1}{2}m\omega^2\mymean{g_m}{x^2}{g_k}=$$
$$=\frac{\hbar\omega}{2}\myint{g_m}{g_k} - \frac{1}{2m}\mymean{g_m}{(-m\omega x + \xi_k)^2}{g_k} + \frac{1}{2}m\omega^2\mymean{g_m}{x^2}{g_k}=$$
$$=\left(\frac{\hbar\omega}{2}-\frac{\xi_k^2}{2m}\right)\myint{g_m}{g_k}+\omega\xi_k\mymean{g_m}{x}{g_k}-%
	 \frac{1}{2}m\omega^2\mymean{g_m}{x^2}{g_k} + \frac{1}{2}m\omega^2\mymean{g_m}{x^2}{g_k}=$$
$$=\left(\left(\frac{\hbar\omega}{2}-\frac{\xi_k^2}{2m}\right)+\omega\xi_k\frac{(\xi_m^*+\xi_k)}{2m\omega}\right)\myint{g_m}{g_k}=%
   \left(\frac{\hbar\omega}{2}+\frac{\xi_m^*\xi_k}{2m}\right)\myint{g_m}{g_k}$$
$$\mathbbm{H}_{mk} - i\hbar\boldsymbol{\tau}_{mk} = \left( \frac{\hbar\omega}{2} + \frac{\xi_m^*\xi_k}{2m} + %
							   \frac{1}{2}m\omega^2q_k^2- \frac{p_k^2}{2m} -\frac{\xi_m^*\xi_k}{2m} \right)\myint{g_m}{g_k}=$$
$$=\left( \frac{\hbar\omega}{2} + \frac{1}{2}m\omega^2q_k^2 - \frac{p_k^2}{2m} \right)\mathbbm{S}_{mk}$$
$$( -i\mathbbm{S}^{-1}\left(\mathbbm{H}-i\hbar\boldsymbol{\tau}\right) )_{nk} = %
    -i\sum_m \mathbbm{S}^{-1}_{nm}\left( \mathbbm{H}_{mk} - i\hbar\boldsymbol{\tau}_{mk} \right) = $$
$$=-i\left( \frac{\hbar\omega}{2} +\frac{1}{2}m\omega^2q_k^2 - \frac{p_k^2}{2m} \right)\sum_m\mathbbm{S}^{-1}_{nm}\mathbbm{S}_{mk} = %
   -i\left( \frac{\hbar\omega}{2} +\frac{1}{2}m\omega^2q_k^2 - \frac{p_k^2}{2m} \right)\delta_{nk}$$
$$\dot{C}_n = -\frac{i}{\hbar}\sum_k \left(\frac{\hbar\omega}{2}+\frac{1}{2}m\omega^2q_k^2-\frac{p_k^2}{2m}\right)\delta_{nk}C_k=%
	      -\frac{i}{\hbar}\left(\frac{\hbar\omega}{2}+\frac{1}{2}m\omega^2q_n^2-\frac{p_n^2}{2m}\right)C_n$$
$$C_n(t) = C_n(0)\ \myexp{-\frac{i}{\hbar}\int_0^t\left(\frac{\hbar\omega}{2}+\frac{1}{2}m\omega^2q_n^2-\frac{p_n^2}{2m}\right)\,dt'}$$
